SStructTT/SStruct/Runtime/Step.lean
@@ -86,20 +86,6 @@ inductive Step0 : State Srt -> State Srt -> Prop where
     Drop H1 m H2 ->
     Step0 (H1, .drop m n) (H2, n)
 
-/- Force alloc-reductions to have deterministic eval order.  -/
-@[simp]def measure : Tm Srt -> Nat
-  | .var _ => 0
-  | .lam _ _ => 1
-  | .app m n => measure m + measure n
-  | .tup m n _ => measure m + measure n + 1
-  | .prj m _ => measure m
-  | .tt => 1
-  | .ff => 1
-  | .ite m _ _ => measure m
-  | .drop _ m => measure m + 1
-  | .ptr _ => 0
-  | .null => 0
-
 /- Alloc-reductions. -/
 @[scoped aesop safe [constructors]]
 inductive Step1 : State Srt -> State Srt -> Prop where
@@ -182,12 +168,13 @@ inductive Step2 : State Srt -> State Srt -> Prop where
     HLookup H l .ff H' ->
     Step2 (H, .ite (.ptr l) n1 n2) (H', n2)
 
-abbrev Red0 (t1 t2 : State Srt) : Prop := Star Step0 t1 t2
-abbrev Red1 (t1 t2 : State Srt) : Prop := Star Step1 t1 t2
+def Red0 (t1 t2 : State Srt) : Prop := Star Step0 t1 t2
+def Red1 (t1 t2 : State Srt) : Prop := Star Step1 t1 t2
+def Step01 (x y : State Srt) : Prop := Star (Union Step0 Step1) x y
 
 inductive Step (x z : State Srt) : Prop where
   | intro {y : State Srt} :
-    Star (Union Step0 Step1) x y -> measure y.2 = 0 -> Step2 y z -> Step x z
+    Step01 x y -> Normal Step01 y -> Step2 y z -> Step x z
 
 notation:50 t:50 " ~>> " t':51 => Step t t'
 notation:50 t:50 " ~>>* " t':51 => Star Step t t'
